src/PlutusIR/Semantics/Static/Normalisation/Strong_Normalisation/SN_STLC/SN_STLC_GU/SN_STLC_GU.v
@@ -1,4 +1,4 @@
-From mathcomp Require Import ssreflect ssrbool eqtype ssrnat.
+From mathcomp Require Import ssreflect ssrbool eqtype.
 From Coq Require Import ssrfun.
 Require Import Coq.Strings.String.
 Require Import Coq.Lists.List.
@@ -6,9 +6,6 @@ From PlutusCert Require Import Util.List Util.
 Import ListNotations.
 Local Open Scope string_scope.
 Local Open Scope list_scope.
-Require Import Lia.
-Require Import Coq.Program.Basics.
-Require Import Coq.Arith.Arith.
 
 Set Implicit Arguments.
 Unset Strict Implicit.
@@ -16,7 +13,6 @@ Unset Printing Implicit Defensive.
 From PlutusCert Require Import alpha_vacuous construct_GU_R alpha_sub psubs step_gu alpha_typing STLC STLC_Kinding SN_STLC_GU.GU_NC_BU SN_STLC_GU.construct_GU.
 From PlutusCert Require Import IdSubst step_naive alpha.alpha alpha_rename rename util alpha_ctx_sub variables alpha_freshness.
 
-(* used to be prop (TODO: Defined also in SN_STCL_named )*)
 Inductive sn {X : Type} {e : X -> X -> Type } x : Type :=
 | SNI : (forall y, e x y -> sn y) -> sn x.
 
@@ -55,69 +51,43 @@ Proof.
   eapply sn_preimage_α'; eauto with α_eq_db.
 Qed.
 
-Create HintDb to_GU'_db.
-Hint Resolve to_GU'__alpha to_GU'__GU to_GU'__NC : to_GU'_db.
-
-Create HintDb to_GU_db.
-Hint Resolve to_GU__alpha to_GU__GU : to_GU_db.
-
 (* This would NOT work for app because of beta reduction*)
 Lemma sn_ty_fun {B s t} : B <> App -> SN_gu s -> SN_gu t -> SN_gu (@tmbin B s t).
-Proof.
+Proof with eauto with gu_nc_db α_eq_db to_GU_db.
   intros HnotApp HSN_s HSN_t.
   generalize dependent t.
   induction HSN_s.
-
   (* now the other IH *)
   intros t.
   elim=> {}. intros.
-
   apply: SNI => y H.
   inversion H; subst.
   inversion H0; subst.
   inversion H2; subst.
   - (* B not App : contradiction *)
     contradiction.
-  - eapply step_naive_preserves_alpha2 with (s' := to_GU x) (R := nil) in H7 as [C [Hstep_C Ha_C] ]; eauto with gu_nc_db α_eq_db to_GU_db.
-    eapply α_preserves_SN_R with (R := []) (s := @tmbin B C t2); eauto with α_eq_db.
+  - eapply step_naive_preserves_alpha2 with (s' := to_GU x) (R := nil) in H7 as [C [Hstep_C Ha_C] ]...
+    eapply α_preserves_SN_R with (R := []) (s := @tmbin B C t2)...
     eapply X with (y := C).
-    + apply step_gu_intro with (s' := to_GU x); eauto with gu_nc_db α_eq_db to_GU_db.
-    + eapply α_preserves_SN_R with (s := x0). eauto. constructor. auto.
-  - eapply step_naive_preserves_alpha2 with (s' := to_GU x0) (R := nil) in H7 as [C [Hstep_C Ha_C] ]; eauto with gu_nc_db α_eq_db to_GU_db.
-    eapply α_preserves_SN_R with (R := []) (s := @tmbin B x C); eauto with α_eq_db.
+    + apply step_gu_intro with (s' := to_GU x)...
+    + eapply α_preserves_SN_R... constructor; auto.
+  - eapply step_naive_preserves_alpha2 with (s' := to_GU x0) (R := nil) in H7 as [C [Hstep_C Ha_C] ]...
+    eapply α_preserves_SN_R with (R := []) (s := @tmbin B x C)...
     eapply X0 with (y := C).
-    apply step_gu_intro with (s' := to_GU x0); eauto with to_GU_db.
+    apply step_gu_intro with (s' := to_GU x0)...
 Qed.
 
 Lemma sn_ty_forall {B X K T} : SN_gu T -> SN_gu (@tmabs B X K T).
-Proof.
-  intros HSN_T.
-  induction HSN_T.
-  apply SNI.
-  intros y Hstep.
+Proof with eauto with α_eq_db gu_nc_db to_GU_db.
+  induction 1.
+  apply SNI; intros y Hstep.
   inversion Hstep; subst.
   inversion H; subst.
   inversion H1; subst.
-
-  eapply step_naive_preserves_alpha2 with (s' := to_GU x) (R := ((y0, X)::nil)) in H7 as [C [Hstep_C Hα_C] ].
-  - 
-    assert (Alpha [] (@tmabs B y0 K s0) (@tmabs B X K C) * step_gu x C)%type as [Hα Hstep_BForall].
-    {
-      split.
-      - constructor; eauto.
-      - apply step_gu_intro with (s' := to_GU x); eauto.
-        + eapply to_GU__alpha.
-        + eapply to_GU__GU.
-    }
-    eapply α_preserves_SN_R with (R := []) (s := @tmabs B X K C) in X0; eauto.
-    eauto with α_eq_db.
-  
-  - eapply gu_lam. eauto.
-  - eapply to_GU__GU.
-  - eapply @alpha_trans with (t := x).
-    + repeat constructor.
-    + eauto with α_eq_db.
-    + eapply alpha_extend_ids. constructor. constructor. apply to_GU__alpha.
+  eapply step_naive_preserves_alpha2 with (s' := to_GU x) (R := ((y0, X)::nil)) in H7 as [C [Hstep_C Hα_C] ]...
+  - eapply α_preserves_SN_R with (R := []) (s := @tmabs B X K C) in X0...
+    apply step_gu_intro with (s' := (to_GU x))...
+  - eapply @alpha_trans with (t := x)...
 Qed.
 
 Lemma sn_closedL {B} t s : SN_gu (@tmbin B s t) -> SN_gu s.
@@ -130,289 +100,178 @@ Qed.
 (* s -> t   ==>  [p/x] s -> [p/x] t*)
 Lemma step_subst_single R {x p s t t' } :
   step_naive s t -> 
-  GU s ->  (*  We could return them, but we don't want to. Current idea: have GU in NC *)
-  NC s [(x, p)] -> (* no free vars in sigma are binders in s'*)
+  GU s -> 
+  NC s [(x, p)] -> 
   Alpha R t t' -> 
   αCtxSub R [(x, p)] [(x, p)] -> 
-  (* GU t' -> *)
   NC t' [(x, p)] ->
   {aT : term & 
   (step_gu (psubs ((x, p)::nil) s) aT) * (Alpha R aT (psubs ((x, p)::nil) t'))}%type.
-Proof with eauto with sconstr2_db.
+Proof with eauto with sconstr2_db gu_nc_db α_eq_db to_GU_db to_GU''_db.
   intros. rename H into Hstep. generalize dependent t'. generalize dependent R. induction Hstep; intros.
-  - 
-    (* The difficult case. The whole reason we need to do global uniqueness every step
-      *)
-      
-
-      assert ({x' : string & {s' & { t' & ((to_GU (@tmbin App (@tmabs Lam x0 A (psubs [(x, p)] s))
-  (psubs [(x, p)] t))) = @tmbin App (@tmabs Lam x' A s') t') * Alpha ((x0, x')::nil) (psubs [(x, p)] s) s' * Alpha [] (psubs [(x, p)] t) t'} } }%type).
-      {
-        eapply to_GU_applam_unfold. auto.
-      }
-      destruct H as [x0' [sub_s [ sub_t [ [pr_eq Ha_subs] Ha_subt]]]].
-      
-      exists (sub x0' sub_t sub_s).
-      split.
-      + eapply step_gu_intro with (s' := (tmbin (tmabs x0' A sub_s) sub_t)).
-        * constructor. constructor. auto. auto.
-        * rewrite <- pr_eq. apply to_GU__GU.
-        * apply step_beta.
-      + (* Invert some stuff to end up with a single sub 
-          We need to freshen s t and p to be able to use commute subst
-        *)
-        remember (sconstr2 x0 t x p s ) as sconstr2_.
-        destruct sconstr2_ as [ [s' t'0] p'].
-
-        eapply @alpha_trans with (ren := ctx_id_left R) (ren' := R) 
-            (t := sub x0 (psubs ((x, p')::nil) t'0) (psubs ((x, p')::nil) s')).
-        * eapply id_left_trans.
-        * eapply alpha_extend_ids.
-          eapply ctx_id_left_is_id.
-
-          eapply alpha_rename_binder_stronger with (Rs := ((x0', x0)::nil)).
-          -- eapply @alpha_trans with (t := psubs ((x, p)::nil) s) (ren := ((x0', x0)::nil)).
-            ++ eapply id_right_trans.
-            ++ eauto with α_eq_db.
-            ++ eapply alpha_extend_ids. constructor. constructor.
-               repeat rewrite psubs_to_subs; try apply single_parseq.
-               eapply psubs__α.
-               ** apply (nc_lam (nc_app_l H1)).
-               ** eapply sconstr2_nc_s. eauto.
-               ** eapply sconstr2_alpha_s. eauto.
-               ** constructor. constructor. constructor. eapply sconstr2_alpha_p. eauto.            
-          -- eapply @alpha_trans with (t := psubs ((x, p)::nil) t).
-              ++ constructor.
-              ++ eauto with α_eq_db.
-              ++ repeat rewrite psubs_to_subs; try apply single_parseq.
-                 eapply psubs__α.
-                 ** apply (nc_app_r H1).
-                 ** eapply sconstr2_nc_t. eauto.
-                 ** eapply sconstr2_alpha_t. eauto.
-                 ** constructor. constructor. constructor. eapply sconstr2_alpha_p. eauto.
-          -- constructor.
-          -- eapply gu_applam_to_nc. rewrite <- pr_eq. apply to_GU__GU.
-          -- repeat rewrite psubs_to_subs; try apply single_parseq.
-             eapply sconstr2_nc_sub; eauto.
-        * 
-        repeat rewrite psubs_to_subs; try apply single_parseq.
-        {
-          eapply commute_sub_naive; eauto.
-          * eapply @alpha_trans with (ren := ctx_id_left R) (ren' := R) (t := sub x0 t s).
-            - eapply id_left_trans.
-            - eapply alpha_extend_ids.
-              eapply ctx_id_left_is_id.
-              repeat rewrite <- single_subs_is_psub.
-              eapply psubs__α with (R := nil).
-              + eapply sconstr2_nc_s_t; eauto.
-              + eapply gu_applam_to_nc. eauto.
-              + eapply @alpha_sym. constructor. eapply sconstr2_alpha_s; eauto.
-              + constructor. constructor. constructor. eapply @alpha_sym. constructor. eapply sconstr2_alpha_t. eauto.
-            - assumption.
-          * eapply αctx_trans with (R1 := ctx_id_left R) (R2 := R) (R := R) (σ' := ((x, p)::nil)); auto.
-            - eapply id_left_trans.
-            - constructor. constructor. 
-              + apply alphavar_extend_ids. apply ctx_id_left_is_id. constructor.
-              + apply alpha_extend_ids. apply ctx_id_left_is_id. eapply @alpha_sym. constructor. eapply sconstr2_alpha_p. eauto.
-          * apply nc_ftv_env with (x := x0) in H1. simpl in H1. simpl. intuition. unfold btv. left. reflexivity.
-          * intros.
-            intros Hcontra.
-            simpl in H.
-            destruct H; auto.
-            rewrite <- H in *.
-            
-            apply nc_ftv_env with (x := x0) in H1.
-            - simpl in H1.
-              destruct H1.
-              right.
-              apply @alpha_preserves_ftv with (ren := nil) (x' := x0) (s' := p) in Hcontra.
-              + auto with *.
-              + eapply @alpha_sym. constructor. eapply sconstr2_alpha_p. eauto.
-              + constructor.
-            - simpl. intuition.
-          * eapply sconstr2_nc_s_t. eauto.
-          * eapply sconstr2_nc_s. eauto.
-          * eapply sconstr2_nc_t. eauto.
-          * eapply sconstr2_nc_sub; eauto.
-        }
-  - inversion H2; subst.
-    
-    
-    specialize (IHHstep (gu_app_l H0) (nc_app_l H1) R H3 s3 H9 (nc_app_l H4)) as [sigS1 [HstepS1 HalphaS1] ].
-
-    inv HstepS1.
-
-    remember (to_GU (@tmbin B s' (psubs ((x, p)::nil) t))) as st_gu.
-    
-    destruct (to_GU_app_unfold Heqst_gu) as [sigS1Alpha [sigtalpha [ [Happ Ha_s] Ha_t ] ] ].
-
-    (* like lam case, we then alpha step *)
-    assert ({s''step & step_naive sigS1Alpha s''step * Alpha [] sigS1 s''step}%type).
+  - (* The difficult case. The whole reason we need to do global uniqueness every step *)
+    (* Globally uniquified version of the termt to step is of the same shape: tmbin (tmabs ...) ...*)
+    assert ({x' : string & {s' & { t' & 
+      ((to_GU (@tmbin App (@tmabs Lam x0 A (psubs [(x, p)] s)) (psubs [(x, p)] t))) = @tmbin App (@tmabs Lam x' A s') t') 
+        * Alpha ((x0, x')::nil) (psubs [(x, p)] s) s' * Alpha [] (psubs [(x, p)] t) t'} } }%type).
     {
-      eapply step_naive_preserves_alpha2 with (s := s') (t := sigS1); eauto.
-      - eapply gu_app_l; eauto.
-        rewrite Heqst_gu in Happ.
-        rewrite <- Happ.
-        eapply to_GU__GU.
+      eapply to_GU_applam_unfold. auto.
     }
-    destruct H7 as [s''step [Halpha_s'' Hstep_s'' ] ].
+    destruct H as [x0' [sub_s [ sub_t [ [pr_eq Ha_subs] Ha_subt]]]]; subst.
+    
+    exists (sub x0' sub_t sub_s). (* Instantiate with ingredients of globally unique term*)
+    split.
+    + eapply step_gu_intro with (s' := (tmbin (tmabs x0' A sub_s) sub_t)).
+      * constructor. constructor. auto. auto.
+      * rewrite <- pr_eq. apply to_GU__GU.
+      * apply step_beta.
+    + (* Freshen s t and p to be able to use commute subst *)
+      remember (sconstr2 x0 t x p s ) as sconstr2_.
+      destruct sconstr2_ as [ [s' t'0] p'].
+
+      eapply @alpha_trans with (ren := ctx_id_left R) (ren' := R) 
+          (t := sub x0 (psubs ([(x, p')]) t'0) (psubs ([(x, p')]) s')); eauto with α_eq_db_trans...
+      * eapply alpha_extend_ids.
+        eapply ctx_id_left_is_id.
+
+        eapply alpha_rename_binder_stronger with (Rs := ((x0', x0)::nil)); eauto...
+        -- eapply @alpha_trans with (t := psubs ((x, p)::nil) s) (ren := ((x0', x0)::nil)); eauto with α_eq_db.
+           eapply alpha_extend_ids. constructor. constructor.
+           eapply psubs__α; eauto with gu_nc_db sconstr2_db α_eq_db.
+        -- eapply @alpha_trans with (t := psubs ((x, p)::nil) t); eauto with α_eq_db.
+           eapply psubs__α...
+        -- constructor.
+        -- eapply gu_applam_to_nc. rewrite <- pr_eq. apply to_GU__GU.
+      * eapply commute_sub_naive; eauto...
+        -- eapply @alpha_trans with (ren := ctx_id_left R) (ren' := R) (t := sub x0 t s); eauto with α_eq_db_trans.
+           eapply alpha_extend_ids.
+           eapply ctx_id_left_is_id.
+           repeat rewrite <- single_subs_is_psub.
+           eapply psubs__α with (R := nil)...
+        -- eapply αctx_trans with (R1 := ctx_id_left R) (R2 := R) (R := R) (σ' := ((x, p)::nil)); auto; eauto with α_eq_db_trans.
+           constructor. constructor. 
+           ++ apply alphavar_extend_ids. apply ctx_id_left_is_id. constructor.
+           ++ apply alpha_extend_ids... apply ctx_id_left_is_id. 
+        -- apply nc_ftv_env with (x := x0) in H1. simpl in H1. simpl. intuition. unfold btv. left. reflexivity.
+        -- intros ftvs HftvsIn Hcontra.
+           destruct HftvsIn; auto.
+           rewrite <- H in *.
+           apply nc_ftv_env with (x := x0) in H1; simpl; auto with *.
+           destruct H1.
+           apply @alpha_preserves_ftv with (ren := nil) (x' := x0) (s' := p) in Hcontra...
+           right; auto with *.
+  - inversion H2; subst.
+    edestruct IHHstep as [sigS1 [HstepS1 HalphaS1] ]...
+    inv HstepS1.
+    remember (to_GU (@tmbin B s' (psubs ((x, p)::nil) t))) as st_gu.
+    destruct (to_GU_app_unfold Heqst_gu) as [sigS1Alpha [sigtalpha [ [Happ Ha_s] Ha_t ] ] ]; subst.
+    eapply step_naive_preserves_alpha2 with (s := s') (s' := sigS1Alpha) (t := sigS1) 
+      in H6 as [s''step [Halpha_s'' Hstep_s'' ] ]...
+    2: eapply gu_app_l; eauto; rewrite <- Happ; apply to_GU__GU.
 
     exists (@tmbin B s''step sigtalpha).
     split.
-    + econstructor; auto.
-      * constructor.
-        -- eapply @alpha_trans. constructor. eauto. eauto.
-        -- eauto.
-      * eauto. subst. rewrite <- Happ. apply to_GU__GU.
+    + apply step_gu_intro with (s' := (@tmbin B sigS1Alpha sigtalpha )); auto...
+      * subst. rewrite <- Happ. apply to_GU__GU.
       * constructor. eauto.
     + eapply @alpha_trans with (ren := ctx_id_left R) (ren' := R). 
       * eapply id_left_trans. 
       * apply alpha_extend_ids. apply ctx_id_left_is_id. constructor. eapply alpha_sym. constructor. eauto. eapply alpha_sym. constructor. eauto.
-      * 
-        constructor. eauto. 
-        repeat rewrite psubs_to_subs; try apply single_parseq.
-        eapply psubs__α; eauto.
-        -- exact (nc_app_r H1).
-        -- exact (nc_app_r H4).
+      * constructor. eauto. 
+        eapply psubs__α; eauto...
   - (* TODO: cleanup, because this is completely analogous to case above*) 
     inversion H2; subst.
-    specialize (IHHstep (gu_app_r H0) (nc_app_r H1) R H3 t3 H10 (nc_app_r H4)) as [sigS1 [HstepS1 HalphaS1] ].
-    repeat rewrite subs_tmbin.
+    edestruct IHHstep as [sigS1 [HstepS1 HalphaS1] ]...
     inv HstepS1.
-
     remember (to_GU (@tmbin B s' (psubs ((x, p)::nil) s))) as st_gu.
-    
-    destruct (to_GU_app_unfold Heqst_gu) as [sigS1Alpha [sigtalpha [ [Happ Ha_s] Ha_t ] ] ].
+    destruct (to_GU_app_unfold Heqst_gu) as [sigS1Alpha [sigtalpha [ [Happ Ha_s] Ha_t ] ] ]; subst.
+    eapply step_naive_preserves_alpha2 with (s := s') (s' := sigS1Alpha) (t := sigS1) 
+      in H6 as [s''step [Halpha_s'' Hstep_s'' ] ]...
+    2: eapply gu_app_l; eauto; rewrite <- Happ; apply to_GU__GU.
 
-    (* like lam case, we then alpha step *)
-    assert ({s''step & step_naive sigS1Alpha s''step * Alpha [] sigS1 s''step}%type).
-    {
-      eapply step_naive_preserves_alpha2 with (s := s') (t := sigS1); eauto.
-      - eapply gu_app_l; eauto.
-        rewrite Heqst_gu in Happ.
-        rewrite <- Happ.
-        eapply to_GU__GU.
-    }
-    destruct H7 as [s''step [Halpha_s'' Hstep_s'' ] ].
-
-    exists (@tmbin B sigtalpha s''step).
-    split.
-    + econstructor; auto.
-      * constructor.
-        -- eauto.
-        -- eapply @alpha_trans. constructor. eauto. eauto.
-        
-      * apply gu_app_st__gu_app_ts. rewrite <- Happ. rewrite Heqst_gu. apply to_GU__GU.
-      * constructor. eauto.
-    + eapply @alpha_trans with (ren := ctx_id_left R) (ren' := R) (t := tmbin (psubs ((x, p)::nil) s) (sigS1)). 
+    exists (@tmbin B sigtalpha s''step); split.
+    + apply step_gu_intro with (s' :=  (@tmbin B sigtalpha sigS1Alpha))...
+      * apply gu_app_st__gu_app_ts. rewrite <- Happ. apply to_GU__GU.
+      * constructor; auto.
+    + eapply @alpha_trans with (ren := ctx_id_left R) (ren' := R) (t := tmbin (psubs ((x, p)::nil) s) (sigS1)).
       * eapply id_left_trans. 
-      * apply alpha_extend_ids. apply ctx_id_left_is_id. constructor. eapply alpha_sym. constructor. eauto. eapply alpha_sym. constructor. eauto.
-      * constructor; eauto. 
-        repeat rewrite psubs_to_subs; try apply single_parseq.
-        eapply psubs__α; eauto.
-        -- exact (nc_app_l H1).
-        -- exact (nc_app_l H4).
+      * apply alpha_extend_ids... apply ctx_id_left_is_id. 
+      * constructor; auto.
+        eapply psubs__α; eauto...
   - inversion H2; subst.
-    specialize (IHHstep (gu_lam H0)).
-
-    assert (HctxSub: αCtxSub ((x0, y)::R) ((x, p)::nil) ((x, p)::nil)).
-    {
-      apply alpha_ctx_ren_extend_fresh_ftv.
-      - apply nc_ftv_env with (x := x0) in H1. auto. simpl. auto.
-      - apply nc_ftv_env with (x := y) in H4. auto. simpl. auto.
-      - assumption.
-    }
-
-    specialize (IHHstep (nc_lam H1) ((x0, y)::R) HctxSub s3 H10 (nc_lam H4)).
-    destruct IHHstep as [subSigmaS2 [Hsteps1 Halpha] ].
-
-    inversion Hsteps1; subst.
-
-    (* Same term, but rename (possibly occuring) x binders to something else, 
-        so that we get GU with the wrapping tmabs x still
-      This should be seen as a composability argument. GU composes up to alpha
-    *)
-    remember (to_GU'' x0 s') as s''.
-
-    (* alpha preserves step_naive, so that we can use this new s'' from above*)
-    assert ({s''step & step_naive s'' s''step * Alpha [] subSigmaS2 s''step }%type).
-    {
-      eapply step_naive_preserves_alpha2 with (s := s'); eauto.
-      - apply @gu_lam with (B := B) (x := x0) (A := A); eauto.
-        subst.
-        eapply to_GU''__GU_lam.
-      - subst.
-        eapply to_GU''__alpha.
-    }
-    destruct H7 as [s''step [Halpha_s'' Hstep_s'' ] ].
-    exists (@tmabs B x0 A s''step).
-    split.
-    + apply step_gu_intro with (s' := @tmabs B x0 A s''); auto. 
-      * constructor.
-        apply alpha_extend_ids. constructor. constructor.
-        eapply @alpha_trans. constructor. eauto. eauto.
-        subst. eapply to_GU''__alpha.
-      * subst. eapply to_GU''__GU_lam.
-      * constructor. assumption.
-    + constructor.
-      eapply @alpha_trans with (ren := ctx_id_left ((x0, y)::R)) (ren' := ((x0, y)::R)).
-      * eapply id_left_trans.
-      * apply alpha_extend_ids. apply ctx_id_left_is_id. eapply @alpha_sym. eauto. constructor. eauto.
+    edestruct IHHstep with (t' := s3) (R := ((x0, y)::R)) as [subSigmaS2 [Hsteps1 Halpha] ]...
+    + apply alpha_ctx_ren_extend_fresh_ftv.
+      * apply nc_ftv_env with (x := x0) in H1. auto. simpl. auto.
+      * apply nc_ftv_env with (x := y) in H4. auto. simpl. auto.
       * assumption.
+    + inversion Hsteps1 as [? ? ? ? ? Hstep_na]; subst.
+      (* Uniquify s' s.t. x0 not used as binder: Composability: GU composes up to alpha *)
+      eapply step_naive_preserves_alpha2 with (s' := to_GU'' x0 s') in Hstep_na as [s''step [Halpha_s'' Hstep_s'' ] ]; eauto...
+      exists (@tmabs B x0 A s''step).
+      split.
+      * apply step_gu_intro with (s' := @tmabs B x0 A (to_GU'' x0 s')); eauto...
+        -- subst. eapply to_GU''__GU_lam.
+        -- constructor; assumption.
+      * constructor.
+        eapply @alpha_trans with (ren := ctx_id_left ((x0, y)::R)) (ren' := ((x0, y)::R))...
+        -- eapply id_left_trans.
+        -- apply alpha_extend_ids... apply ctx_id_left_is_id. 
 Qed.
 
 Definition sub_gu (X : string) (T : term) (s : term) := sub X T (to_GU' X T s).
 
 Lemma sn_subst X T s : NC s ((X, T)::nil) -> SN_gu (sub X T s) -> SN_gu s.
 Proof with eauto with to_GU'_db.
-  intros nc.
-  assert (Alpha [] (sub X T s) (sub X T (to_GU' X T s))).
-  {
-    repeat rewrite <- single_subs_is_psub.
-    eapply psubs__α; eauto.
-    eapply to_GU'__NC.
-    eapply to_GU'__alpha.
-    constructor. constructor. constructor. apply alpha_refl. constructor.
-  }
-  (* intros.
-  eapply α_preserves_SN_R with (R := nil) (s := (to_GU' X T s)).
-  - eapply @alpha_sym; auto. constructor. apply to_GU'__alpha.
-  -  *)
-  intros.
-    rewrite <- single_subs_is_psub in X0.
-    eapply α_preserves_SN_R with (s := psubs ((X, T)::nil) s) (s' := psubs((X, T)::nil) (to_GU' X T s)) in X0.
-    {
-      rewrite single_subs_is_psub in X0.
-      revert X0.
-      
-    apply (sn_preimage_α (h := sub_gu X T)) => x y. 
-    intros.
-    (* eapply (@step_gu_preserves_alpha) with (R := nil) (t := to_GU' X T x) in H1... (* so that we already have a GU term*)
-    destruct H1 as [t' [Hstep H_a] ]. *)
-    (* to_GU' is created such that we have GU s and NC s ((X, T))*)
-    unfold sub_gu.
-    repeat rewrite <- single_subs_is_psub.
-    inversion H0; subst.
-    eapply step_naive_preserves_alpha2 with (R := nil) (t:= y) (s' := to_GU' X T x) in H3; auto with α_eq_db.
-    {
-      destruct H3 as [t'' [Hstep_t'' Ha_t''] ].
-      eapply @step_subst_single with (s := (to_GU' X T x)) (t := t''); eauto...
-      - apply @alpha_trans with (t := y) (ren := nil) (ren' := nil); repeat constructor...
-        eauto with α_eq_db.
-      - eauto with α_eq_db.
-    }
-    - apply to_GU'__GU.
-    - eapply @alpha_trans with (t := x); eauto with α_eq_db. apply to_GU'__alpha.
-  }
-  eapply psubs__α with (R := nil); eauto.
-  - apply to_GU'__NC.
-  - apply to_GU'__alpha.
-  - constructor. constructor. constructor. apply alpha_refl. constructor.
+  intros Hnc HSN_sub.
+  rewrite <- single_subs_is_psub in HSN_sub.
+  eapply α_preserves_SN_R with (s := psubs ((X, T)::nil) s) (s' := psubs((X, T)::nil) (to_GU' X T s)) 
+    in HSN_sub; eauto using psubs__α with α_eq_db...
+  2: eapply psubs__α with (R := nil); eauto with α_eq_db...
+  rewrite single_subs_is_psub in HSN_sub.
+  revert HSN_sub.
+  apply (sn_preimage_α (h := sub_gu X T)) => x y Hstep.
+  unfold sub_gu.
+  repeat rewrite <- single_subs_is_psub.
+  inversion Hstep; subst.
+  eapply step_naive_preserves_alpha2 with (R := nil) (t:= y) (s' := to_GU' X T x) 
+    in H1 as [t'' [Hstep_t'' Ha_t''] ]; eauto with α_eq_db...
+  2: eapply @alpha_trans with (t := x); eauto with α_eq_db...
+  eapply @step_subst_single with (s := (to_GU' X T x)) (t := t''); eauto with α_eq_db...
+  apply @alpha_trans with (t := y) (ren := nil) (ren' := nil); repeat constructor...
+  eauto with α_eq_db.  
+Qed.
+
+Lemma red_beta x s t1 t2 : 
+  step_gu t1 t2 ->
+  NC s ((x, t1)::nil) ->
+  { a & prod 
+    ( red_gu_na (sub x t1 s) a) 
+    ( nil ⊢ a ~ sub x t2 s) }. 
+Proof with eauto with α_eq_db. 
+  intros Hstep HNC_t1.
+  induction s.
+  - eexists; split...
+    destr_eqb_eq x s; simpl.
+    + rewrite String.eqb_refl.
+      apply red_gu_na_star with (t := t2); auto; constructor.
+    + rewrite <- String.eqb_neq in H; rewrite H; constructor.
+  - specialize (IHs (nc_lam HNC_t1)) as [a [Hred_a Ha_a] ].
+    assert ({a0 : term & (red_gu_na (@tmabs USort s k (sub x t1 s0)) a0 *
+                            (nil ⊢ a0 ~ @tmabs USort s k a))%type}) 
+      as [a0 [Hred_a0 Ha_a0]] by apply (red_gu_na_lam_fold Hred_a).
+    eexists; split...
+  - specialize (IHs1 (nc_app_l HNC_t1) ) as [g1 [Hred_g1 ?] ].
+    specialize (IHs2 (nc_app_r HNC_t1) ) as [g2 [Hred_g2 ?] ].
+    assert ({a : term & (red_gu_na (@tmbin BSort (sub x t1 s1) (sub x t1 s2)) a *
+                          (nil ⊢ a ~ @tmbin BSort g1 g2))%type}) 
+      as [app [Hred Ha] ] by apply (red_gu_na_app_fold Hred_g1 Hred_g2).
+    eexists; split...
+  - eexists. split; constructor.
 Qed.
 
 Definition cand := term -> Type.
 
-(* TODO: This is different then neutral_Ty*)
+(* Note: This is different then neutral_Ty*)
 Definition neutral (s : term) : bool :=
   match s with
     | tmabs _ _ _ => false
@@ -430,9 +289,6 @@ match T with
   | PlutusIR.Kind_Base => SN_gu 
   | PlutusIR.Kind_Arrow A B => fun s => forall t, L A t -> L B (@tmbin App s t)
 end.
-
-Create HintDb a_constr_db.
-Hint Resolve a_constr__s_alpha a_constr__t_alpha : a_constr_db.
 
 Lemma α_preserves_L_R A s s' R :
   Alpha R s s' -> L A s -> L A s'.
@@ -461,8 +317,6 @@ Proof.
   intros s.  elim: s => //.
 Qed.
 
-Global Hint Resolve reducible_sn : core.
-
 Lemma reducible_var P x : reducible P -> P (tmvar x).
 Proof. move/p_nc. apply=> // t st.
   inv st. inv H. inv H1.
@@ -484,31 +338,25 @@ Proof with eauto using step_gu.
   - apply reducible_sn.
   - constructor.
     + move=> s h.
-     apply: (@sn_closedL App (tmvar "x")). apply: (p_sn (P := L B))...
+      apply: (@sn_closedL App (tmvar "x")). apply: (p_sn (P := L B))...
       eapply h. eapply reducible_var; eauto.
     + intros. specialize (X t0 X0).
       eapply step_gu_app_l with (s1 := s) (t1 := t) (s2 := t0) in H. 
       * destruct H as [t1' [ Ha_t [s2' [Ha_s2' Hstep] ] ] ].
         eapply p_cl with (s := (tmbin s t0)) in X; auto.
         2: exact Hstep.
-        eapply α_preserves_L_R.
-        2: eauto.
+        eapply α_preserves_L_R; eauto.
         constructor; eapply alpha_sym; eauto; constructor.
     + move=> s ns h t la.
       have snt := p_sn ih1 la.
       elim: snt la => {} t _ ih3 la. apply: p_nc... move=> v st. inv st=> //...
       inv H.  inv H1=> //...
       * inv H7. discriminate ns.
-      * assert (Hgn: step_gu s s0).
-        {
-          apply gu_app_l in H0.
-          econstructor; eauto.
-        }
-        eapply α_preserves_L_R with (s' := t2) in la; eauto.
+      * eapply α_preserves_L_R with (s' := t2) in la; eauto.
+        apply gu_app_l in H0; eauto using step_gu_intro.
       * assert (step_gu t t0).
         {
-          apply gu_app_r in H0.
-          econstructor; eauto.    
+          apply gu_app_r in H0; eauto using step_gu_intro.
         }
         specialize (ih3 t0 H).
         eapply α_preserves_L_R; eauto.
@@ -550,299 +398,146 @@ Proof.
   - assumption.
 Qed.
 
-Definition EL (Gamma : list (string * PlutusIR.kind)) 
-          (sigma : list (string * term)) : Type :=
-  forall x T, lookup x Gamma = Some T ->
-    { t & prod (lookup x sigma = Some t) (L T t)}.
-
-Lemma extend_EL (Gamma : list (string * PlutusIR.kind)) (sigma : list (string * term)) x T t :
-  EL Gamma sigma -> L T t -> EL ((x, T) :: Gamma) ((x, t) :: sigma).
-Proof.
-  intros.
-  unfold EL.
-  intros.
-  destr_eqb_eq x0 x.
-  - exists t.
-    split.
-    + simpl. rewrite String.eqb_refl. reflexivity.
-    + simpl in H. rewrite String.eqb_refl in H. inversion H. subst. assumption.
-  - simpl in H. rewrite <- String.eqb_neq in H0. rewrite String.eqb_sym in H0. rewrite H0 in H.
-    unfold EL in X.
-    specialize (X x0 T0 H).
-    
-    destruct X as [t' [H3 H4] ].
-    exists t'.
-    split.
-    + simpl. rewrite H0. assumption.
-    + assumption.
-Qed.
-
-
-Lemma red_beta x s t1 t2 : 
-  step_gu t1 t2 ->
-  NC s ((x, t1)::nil) ->
-  NC s ((x, t2)::nil) -> (* step does not introduce new free vars, so should be true!*)
-  { a & prod 
-    ( red_gu_na (sub x t1 s) a) 
-    ( nil ⊢ a ~ sub x t2 s) }. 
-Proof with eauto with α_eq_db. 
-  intros Hstep.
-  induction s.
-  - intros.
-    destr_eqb_eq x s.
-    + simpl.
-      rewrite String.eqb_refl.
-      exists t2.
-      split...
-      apply red_gu_na_star with (t := t2); auto.
-      apply red_gu_na_nil.
-    + simpl.
-      rewrite <- String.eqb_neq in H1.
-      rewrite H1.
-      exists (tmvar s).
-      split...
-      apply red_gu_na_nil.
-  - intros.
-    simpl.
-    assert (x <> s).
-    {
-      intros contra.
-      subst.
-      eapply nc_ftv_env with (x := s) in H.
-      + unfold ftv_keys_env in H.
-        contradiction H.
-        apply in_eq.
-      + simpl. apply in_eq.
-    }
-    specialize (IHs (nc_lam H) (nc_lam H0)) as [a [Hred_a Ha_a] ].
-    assert ({a0 : term &
-  (red_gu_na (@tmabs USort s k (sub x t1 s0)) a0 *
-  (nil ⊢ a0 ~ @tmabs USort s k a))%type}).
-  {
-    apply (red_gu_na_lam_fold Hred_a).
-  }
-    destruct H2 as [a0 [Hred_a0 Ha_a0] ].
-    exists a0.
-    split.
-    + assumption.
-    + eapply alpha_trans.
-      * constructor.
-      * eauto.
-      * constructor. eapply alpha_extend_id'; auto. constructor. (* TODO: make that a lemma*)
-  - intros.
-    specialize (IHs1 (nc_app_l H) (nc_app_l H0)) as [g1 [Hred_g1 Ha_g1] ].
-    specialize (IHs2 (nc_app_r H) (nc_app_r H0)) as [g2 [Hred_g2 Ha_g2] ].
-    repeat rewrite <- single_subs_is_sub.
-    repeat rewrite <- single_subs_is_sub in *.
-    repeat rewrite single_subs_is_sub.
-    repeat rewrite single_subs_is_sub in *.
-    
-    assert ({a : term &
-    (red_gu_na
-      (@tmbin BSort (sub x t1 s1) (sub x t1 s2)) a *
-    (nil ⊢ a ~
-    @tmbin BSort g1 g2))%type}) as [app [Hred Ha] ] by apply (red_gu_na_app_fold Hred_g1 Hred_g2).
-    exists app.
-    split; auto.
-    eapply alpha_trans; eauto with α_eq_db.
-  - intros.
-    simpl.
-    exists (tmbuiltin d).
-    split.
-    + constructor.
-    + constructor.
-Qed.
-
-(* Closure under beta expansion. *)
+(* Reverse of beta reduction. *)
 Lemma beta_expansion' {BA BL} A B x y s s' t :
-  Alpha [(y, x)] s' s -> (* this allows us to not have to "rename free vars in t" manually*)
+  Alpha [(y, x)] s' s -> 
   GU s ->
-  NC s [(x, t)] -> (* this really is the right assumption. no free variable in t is a binder in s', because these binders could be added to the environment through beta reduction and then capture*)
+  NC s [(x, t)] -> 
   SN_gu t -> 
   L A (sub x t s) ->
   L A (@tmbin BA (@tmabs BL y B s') t).
 Proof with eauto with α_eq_db gu_nc_db.
-  move=> Ha_s' gu nc snt h. have sns := sn_subst nc (L_sn h).
-  assert (SN_gu s').
-  {
-    (* eapply alpha_sym in Ha_s'. *)
-    eapply α_preserves_SN_R with (s := s)...
+  move=> Ha_s' gu nc snt h.
+  assert (Hsns': SN_gu s').
+  { eapply α_preserves_SN_R with (s := s)... 
+    apply (sn_subst nc (L_sn h)).
   }
-  clear sns.
   generalize dependent s.
   generalize dependent t.
-  induction X.
-  intros t snt s0 Ha Hnc.
-
+  induction Hsns' as [? ? IH1]; intros t snt s0 Ha Hnc.
   (* Now create IH for other step *)
   revert Hnc.
   revert snt.
-  elim=> {}.
-  intros.
-  rename X0 into H10.
+  induction 1 as [? ? IH2]; intros Hgu Hnc HL.
 
   apply: L_nc => // u st. 
-  inversion st; subst. inv H. inversion H7; subst. 
-
+  inversion st; subst. inv H. inversion H7; subst; clear st.
   inv H1 => //.
   - eapply α_preserves_L_R with (R := (nil)); eauto.
-    (* repeat rewrite <- single_subs_is_sub. *)
     eapply alpha_rename_binder_stronger with (Rs := ((x, y0)::nil))...
     constructor.
   - inv H5.
-    assert (Alpha [(y, y0)] (to_GU x0) s4).
+    assert ({s5' & step_naive (to_GU x0) s5' * Alpha [(y0, y)] s5 s5'}%type)
+      as [s5' [Hstep_na_s5' Ha_s5'] ].
     {
-      eapply @alpha_trans with (ren := (y, y)::nil) (t := x0).
-      - eauto with α_eq_db.
-      - apply alpha_extend_ids. constructor. constructor. eapply @alpha_sym; eauto. constructor. apply to_GU__alpha.
-      - assumption.
-    }
-    assert ({s5' & step_naive (to_GU x0) s5' * Alpha [(y0, y)] s5 s5'}%type).
-    {
-
       eapply step_naive_preserves_alpha2 with (s := s4) (t:=s5) (s' := (to_GU x0))...
       apply to_GU__GU.
+      eapply @alpha_trans with (ren' := (y, y)::nil) (t := x0)...
+      apply alpha_extend_ids; eauto with to_GU_db. repeat constructor.
     }
-    destruct H1 as [s5' [Hstep_na_s5' Ha_s5'] ].
-    assert (Hstep_s5': step_gu x0 s5').
-    {
-      apply step_gu_intro with (s' := to_GU x0).
-      - eapply to_GU__alpha.
-      - eapply to_GU__GU.
-      - assumption.
-    }
-
+    eapply step_gu_intro in Hstep_na_s5'; eauto with to_GU_db...
     eapply α_preserves_L_R with (s := tmbin (tmabs y B s5') x1) (R := nil)...
-    specialize (X s5' Hstep_s5' x1).
-    clear Ha_s5'. clear H7. clear st. 
-    inv Hstep_s5'.
-    assert (HSN_x1: SN_gu x1) by now constructor.
-
-    (* TODO: instead of to_GU, assume gu of s0 here by NC?*)
-    assert ({s'_a &  step_naive s0 s'_a * Alpha [(y, x)] s5' s'_a}%type).
-    {
-      eapply step_naive_preserves_alpha2 with (s := s') (s' := s0) (t := s5')...
-      eapply @alpha_trans with (ren := (y, y)::nil) (ren' := (y, x)::nil) (t := x0)...
-    }
-    destruct H4 as [s'_a [ Hstep_s'_a Ha_s'_a ] ].
-    specialize (X HSN_x1 (to_GU' x x1 s'_a)). (* just renaming binders*)
-    remember (to_GU' x x1 s'_a) as s'_a1.
-    assert (((y, x)::nil) ⊢ s5' ~ s'_a1).
-    {
-      eapply @alpha_trans with (ren := ((y, x)::nil)) (ren' := ctx_id_right ((y, x)::nil)) (t := s'_a)...
-      eapply alpha_extend_ids. constructor. constructor. subst. eapply to_GU'__alpha.
-    }
-
-    eapply X; eauto.
-
-    * subst. eapply to_GU'__GU. 
-    * subst. eapply to_GU'__NC.
-    * 
-    assert ({α & (step_gu (sub x x1 s0) α) * (nil ⊢ α ~ sub x x1 s'_a1)}%type) 
-      as [alpha [Hred Halpha] ].
+    specialize (IH1 _ Hstep_na_s5').
+    inv Hstep_na_s5'.
+    edestruct step_naive_preserves_alpha2 with (R := [(y, x)]) (s' := s0) (t := s5') as [s'_a [Hstep_s'_a Ha_s'_a] ]...
+    1: eapply @alpha_trans with (ren := (y, y)::nil) (ren' := (y, x)::nil) (t := x0)...
+    eapply IH1 with (s := (to_GU' x x1 s'_a)); subst; eauto with to_GU'_db α_eq_db...
+    + now constructor.
+    + assert ({α & (step_gu (sub x x1 s0) α) * (nil ⊢ α ~ sub x x1 (to_GU' x x1 s'_a))}%type) 
+        as [alpha [Hred Halpha] ].
       {
         repeat rewrite <- single_subs_is_psub.
-        eapply (@step_subst_single)...
-        subst. eapply to_GU'__alpha.
-        subst. eapply to_GU'__NC.
+        eapply (@step_subst_single); eauto with to_GU'_db...
       }
-    eapply α_preserves_L_R with (s := alpha) (R := nil); auto.
-    eapply L_cl with (s := (sub x x1 s0)); auto.
-
+      eapply α_preserves_L_R with (s := alpha) (R := nil); auto.
+      eapply L_cl with (s := (sub x x1 s0)); auto.
   - eapply α_preserves_L_R with (s := (tmbin (tmabs y B x0) t0)) (R := nil)...
-    eapply H10.
+    eapply IH2; auto.
     + econstructor...
-    + assumption.
     + eapply step_naive_preserves_nc_ctx with (s := s0); eauto.
       eapply alpha_preserves_nc_ctx; eauto.
-    +  
-      assert ({ a & prod 
-    ( red_gu_na (sub x x1 s0) a) 
-    ( nil ⊢ a ~ sub x t0 s0) }).
-      { (* this has a lot of repetition with the above *)
-        apply red_beta...
-        - econstructor...
-        - eapply step_naive_preserves_nc_ctx with (s := s0); eauto.
-          eapply alpha_preserves_nc_ctx; eauto.
-      }
-      destruct H as [a [Hred_a Ha_a] ].
-      eapply (L_cl_star) in h.
-      * eapply α_preserves_L_R with (R := nil); eauto.
-      * assumption.
+    + edestruct red_beta as [a [Hred_a Ha_a]] in H5; eauto.
+      * econstructor... 
+      * eapply (L_cl_star) with (t := a) in HL; auto.
+        eapply α_preserves_L_R with (R := nil); eauto.
+Qed.
+
+Definition EL (Δ : list (string * PlutusIR.kind)) 
+          (sigma : list (string * term)) : Type :=
+  forall x T, lookup x Δ = Some T ->
+    { t & prod (lookup x sigma = Some t) (L T t)}.
+
+Lemma extend_EL (Δ : list (string * PlutusIR.kind)) (sigma : list (string * term)) x T t :
+  EL Δ sigma -> L T t -> EL ((x, T) :: Δ) ((x, t) :: sigma).
+Proof.
+  intros HEL HL.
+  unfold EL. intros x0 T0 Hl.
+  destr_eqb_eq x0 x.
+  - exists t.
+    split; simpl.
+    + rewrite String.eqb_refl. reflexivity.
+    + simpl in Hl. rewrite String.eqb_refl in Hl. inversion Hl. subst. assumption.
+  - simpl in Hl. rewrite <- String.eqb_neq in H. rewrite String.eqb_sym in H. rewrite H in Hl.
+    unfold EL in HEL.
+    specialize (HEL x0 T0 Hl).
+    
+    destruct HEL as [t' [H3 H4] ].
+    exists t'.
+    split; auto.
+    simpl. rewrite H. assumption.
 Qed.
 
 Lemma beta_expansion_subst {BA BL} X t sigma s A B :
   ParSeq ((X, t)::sigma) ->
   NC (psubs sigma s) [(X, t)] -> (* so the substitution makes sense after "breaking"  it open*)
-  SN_gu t -> L A (psubs ((X, t)::sigma) s) -> L A (@tmbin BA (psubs sigma (@tmabs BL X B s)) t).
-Proof.
-  intros HPS nc snt H.
-  simpl in H.
-  eapply α_preserves_L_R with (R := nil) (s := (@tmbin BA (@tmabs BL X B (to_GU' X t (psubs sigma s))) t)).
-  - constructor. constructor. apply alpha_extend_ids. constructor. constructor. 
-    eapply @alpha_sym. eauto. constructor. apply to_GU'__alpha. eapply alpha_refl. constructor.
-  - eapply α_preserves_L_R with (R := nil) (s' := (sub X t (to_GU' X t (psubs sigma s)))) in H.
-    + 
-      eapply beta_expansion' in H; eauto.
-      * apply alpha_extend_ids. constructor. constructor. apply alpha_refl. constructor.
-      * eapply to_GU'__GU.
-      * eapply to_GU'__NC.
+  SN_gu t -> 
+  L A (psubs ((X, t)::sigma) s) -> L A (@tmbin BA (psubs sigma (@tmabs BL X B s)) t).
+Proof with eauto with α_eq_db to_GU'_db.
+  intros HPS nc snt HL.
+  eapply α_preserves_L_R with (R := []) (s := (@tmbin BA (@tmabs BL X B (to_GU' X t (psubs sigma s))) t)).
+  - constructor; eauto...
+  - eapply α_preserves_L_R with (R := []) (s' := (sub X t (to_GU' X t (psubs sigma s)))) in HL.
+    + eapply beta_expansion' in HL; eauto...
     + repeat rewrite <- single_subs_is_psub.
-      assert (psubs ((X, t)::sigma) s = psubs [(X, t)] (psubs sigma s)).
-      {
-        apply psubs_unfold; auto.
-      }
-      rewrite H0.
-      apply psubs__α; auto.
-      * eapply to_GU'__NC.
-      * eapply to_GU'__alpha.
-      * apply alpha_ctx_ren_nil.
+      rewrite psubs_unfold; auto.
+      apply psubs__α; auto...
 Qed.
 
-(* The fundamental theorem. *)
-Theorem soundness Gamma s A :
-  has_kind Gamma s A -> 
+(* The fundamental theorem of L. *)
+Theorem fundamental Δ s A :
+  Δ |-* s : A -> 
   GU s -> (* So that we know GU_vars (tmabs x A s) -> ~ In x (btv s), and btv s ∩ ftv s = ∅, important for dealing with vars in `t` that roll out of LR*)
   forall sigma, 
-    BU sigma s -> (* so btv sigma is disjoint from tv s + ftv_env sigma: Allows adding btvs 
-                        to alpha context without accidentally renaming ftvs*)
-    NC s sigma -> (* so we get "nice" substitutions (is contained in BU) *)
+    BU sigma s -> (* Allows adding btvs to alpha context without accidentally renaming ftvs*)
+    NC s sigma -> (* so we get no capture substitutions *)
     ParSeq sigma -> (* So parallel and sequential substitions are identical *)
-    EL Gamma sigma -> (* So that terms in a substitution are already L *)
+    EL Δ sigma -> (* So that terms in a substitution are already L *)
   L A (psubs sigma s).
-Proof with eauto using L_sn. 
-  elim=> {Gamma s A}.
-  - intros Gamma X A ih gu sigma wierd nc blabla HEL.
+Proof with eauto using L_sn with gu_nc_db bu_db. 
+  elim=> {Δ s A}.
+  - (* K_Var *)
+    intros Δ X A ih gu sigma bu nc ps HEL.
     unfold EL in HEL.
-    specialize (HEL X A ih).
-    destruct HEL as [t [HlookupSigma LAt] ].
-    simpl.
-    rewrite HlookupSigma.
-    assumption.
+    destruct (HEL X A ih) as [t [HlookupSigma LAt] ]; simpl.
+    rewrite HlookupSigma; auto.
   - (* FUN*)
     intros.
     unfold L.
     eapply sn_ty_fun.
     + unfold not. intros Hcontra. inversion Hcontra.
-    + eapply X; eauto with gu_nc_db.
-      eapply BU_appl; eauto.
-    + eapply X0; eauto with gu_nc_db.
-      eapply BU_appr; eauto.
+    + eapply X...
+    + eapply X0...
   - (* IFix *)
     intros.
     unfold L.
     eapply sn_ty_fun.
-    + unfold not. intros Hcontra. inversion Hcontra.
-    + eapply L_sn.
-      eapply X0; eauto with gu_nc_db.
-      eapply BU_appl; eauto.
-    + eapply L_sn.
-      eapply X; eauto with gu_nc_db.
-      eapply BU_appr; eauto.
+    all: try eapply L_sn...
+    unfold not. intros Hcontra. inversion Hcontra.
   - (* Forall *)
     intros.
     unfold L.
     eapply sn_ty_forall.
+    fold psubs.
     assert (psubs sigma T = psubs ((X, tmvar X)::sigma) T).
     {
       apply psubs_extend_new.
@@ -852,31 +547,22 @@ Proof with eauto using L_sn.
     } 
     fold psubs.
     rewrite H3.
-    eapply X0 with (sigma := ((X, tmvar X)::sigma)); eauto with gu_nc_db.
-    + eapply BU_lam_id; eauto.
-    + constructor; auto.
-      * eapply nc_lam; eauto.
-      * intros.
-        destr_eqb_eq y X.
-        -- exfalso.
-           inversion H; subst.
-           contradiction.
-        -- split; auto.
-           unfold ftv. simpl. unfold not. intros Hcontra. intuition.
-    + unfold BU in H0.
-      destruct H0 as [ BU1 BU2].
-      constructor; auto.
-      * assert (~ In X (ftv_keys_env sigma)).
-        {
-          intros contra.
-          eapply nc_ftv_env with (x := X) in H1.
-          contradiction.
-          apply btv_lam.
-        }
-        intros Hcontra.
-        apply ftv_keys_env_sigma_remove in Hcontra. contradiction.
-      * intros Hcontra.
-        apply BU1 in Hcontra; auto.
+    eapply X0 with (sigma := ((X, tmvar X)::sigma)); eauto with gu_nc_db bu_db.
+    + constructor; eauto...
+      intros.
+      destr_eqb_eq y X.
+      -- exfalso.
+         inversion H; subst.
+         contradiction.
+      -- split; auto.
+         unfold ftv. simpl. unfold not. intros Hcontra. intuition.
+    + destruct H0 as [BU1 BU2]. 
+      constructor; auto; intros Hcontra.
+      * apply ftv_keys_env_sigma_remove in Hcontra.
+        eapply nc_ftv_env with (x := X) in H1.
+        contradiction.
+        apply btv_lam.
+      * apply BU1 in Hcontra; auto.
         simpl in Hcontra.
         intuition.
     + eapply extend_EL. eauto. apply L_var.
@@ -886,48 +572,32 @@ Proof with eauto using L_sn.
     constructor.
     intros.
     inv H3. inv H4. inv H6. (* no step from builtin *)
-  - intros Gamma X A s B _ ih gu sigma wierd nc blabla EL.
-    unfold L. fold L.
-    intros.
-
+  - (* K_Lam *)
+    intros Δ X A s B _ ih gu sigma bu nc ps EL.
+    simpl L; intros t HLA.
     remember (t_constr t s sigma X) as t'R.
     destruct t'R as [t' R].
-
     assert (HBU: BU ((X, t')::sigma) s).
-    {
-      eapply BU_lam2; eauto.
-    }
+    { eapply BU_lam2; eauto. }
     assert (HX: ~ In X (btv s)).
-    {
+    { 
       intros contra.
       inversion gu; subst.
       contradiction.
     }
-
-    specialize (ih (gu_lam gu) ((X, t')::sigma) HBU (t_constr__nc_s HX (nc_lam nc) Heqt'R)).
     assert (Hparseq: ParSeq ((X, t')::sigma)).
     {
-      (* we now need: X not a binder in sigma. *)
-      constructor. auto.
-        - assert (~ In X (ftv_keys_env sigma)).
-        {
-          intros contra.
-          eapply nc_ftv_env with (x := X) in nc.
-          contradiction.
-          apply btv_lam.
-        }
-        intros Hcontra.
-        apply ftv_keys_env_sigma_remove in Hcontra. contradiction.
-      - unfold BU in wierd. destruct wierd as [ BU1 _].
-        intros Hcontra.
+      constructor; auto; intros Hcontra.
+      - apply ftv_keys_env_sigma_remove in Hcontra. 
+        apply nc_ftv_env with (x := X) in nc; [|apply btv_lam].
+        contradiction.
+      - destruct bu as [ BU1 _ ].
         apply BU1 in Hcontra; auto.
         simpl in Hcontra.
         intuition.
     }
-
-    specialize (ih Hparseq (extend_EL EL (α_preserves_L_R (t_constr__a_t Heqt'R) X0))).
-  (* **** ih tis now fully applied ********************** *)
-
+    specialize (ih (gu_lam gu) ((X, t')::sigma) HBU (t_constr__nc_s HX (nc_lam nc) Heqt'R) Hparseq (extend_EL EL (α_preserves_L_R (t_constr__a_t Heqt'R) HLA))).
+    (* **** ih is now fully applied ********************** *)
     eapply beta_expansion_subst in ih; auto.
     + eapply α_preserves_L_R with (s' := tmbin (psubs sigma (tmabs X A s)) t) (R := sym_alpha_ctx R) in ih; eauto. constructor.
       * eapply @alpha_sym with (ren := R). apply sym_alpha_ctx_is_sym.
@@ -938,7 +608,7 @@ Proof with eauto using L_sn.
       * eapply @alpha_sym; eauto. apply sym_alpha_ctx_is_sym.   
         apply (t_constr__a_t Heqt'R).
     + eapply t_constr__nc_subs; eauto.
-      unfold BU in wierd. destruct wierd as [ BU1 _ ].
+      destruct bu as [ BU1 _ ].
       intros Hcontra.
       apply BU1 in Hcontra; auto.
       simpl in Hcontra.
@@ -946,57 +616,40 @@ Proof with eauto using L_sn.
     + eapply α_preserves_SN_R; eauto. 
       * eapply t_constr__a_t; eauto. 
       * eapply L_sn; eauto.
-  - intros Gamma s t A B _ ih1 _ ih2 gu sigma wierd nc blabla HEL.
-    specialize (ih1 (gu_app_l gu) sigma).
-
-    specialize (ih1 (BU_appl wierd) (nc_app_l nc) blabla HEL).
-    specialize (ih2 (gu_app_r gu) _ (BU_appr wierd) (nc_app_r nc) blabla HEL).
-    repeat rewrite subs_tmbin.
-    unfold L in ih1. fold L in ih1.
-    specialize (ih1 (psubs sigma t) ih2).
-    assumption.
+  - intros Δ s t A B _ ih1 _ ih2 gu sigma bu nc ps HEL.
+    simpl L in ih1; eauto.
+    apply ih1; eauto with gu_nc_db bu_db.
 Qed.
 
 (* The identity substitution is in the EL relation *)
-Lemma id_subst__EL E :
-  EL E (id_subst E).
+Lemma id_subst__EL Δ :
+  EL Δ (id_subst Δ).
 Proof.
-  induction E.
-  - intros. simpl. unfold EL. intros. inversion H.
-  - intros.
-    destruct a as [x K].
-    simpl.
+  induction Δ; intros; simpl.
+  - unfold EL. intros. inversion H.
+  - destruct a as [x K].
     apply extend_EL; eauto.
     apply L_var.
 Qed.
 
 (* The fundamental theorem for named variables. *)
-Corollary type_L (E : list (string * PlutusIR.kind)) s T : has_kind E s T -> L T (psubs (id_subst E) s).
-Proof.
-  intros Htype.
-  assert (HEL: EL E (id_subst E)) by apply id_subst__EL.
-  remember (s_constr s (id_subst E)) as s'.
-  eapply alpha_preserves_typing with (t := s') (sigma := nil) (Gamma := E) in Htype; eauto.
+Corollary type_L Δ s T : Δ |-* s : T -> L T (psubs (id_subst Δ) s).
+Proof with eauto using id_subst__EL with s_constr_db id_subst_db.
+  intros Hkind.
+  remember (s_constr s (id_subst Δ)) as s'.
+  eapply alpha_preserves_typing with (t := s') (sigma := nil) (Gamma := Δ) in Hkind; eauto...
   {
-    eapply soundness in Htype; eauto.
-    - rewrite id_subst__id in Htype; [|apply id_subst_is_IdSubst]. 
-      rewrite id_subst__id; [|apply id_subst_is_IdSubst].
-      eapply α_preserves_L_R with (s := s'); eauto.
-      eapply alpha_sym. eapply alpha_sym_nil. eapply s_constr__a_s; eauto.
-    - eapply s_constr__gu; eauto.
-    - apply id_subst__nc_BU. eapply s_constr__nc_s; eauto.
-    - eapply s_constr__nc_s; eauto.
-    - apply id_subst__ParSeq. apply id_subst_is_IdSubst.
+    eapply fundamental in Hkind; eauto...
+    - rewrite id_subst__id in Hkind...
+      rewrite id_subst__id...
+      eapply α_preserves_L_R with (s := s'); eauto with α_eq_db s_constr_db.
   }
-  - eapply s_constr__a_s; eauto.
-  - constructor.
+  constructor.
 Qed.
 
-Theorem SN_gu' E s T : has_kind E s T -> @sn term step_gu s.
-  intros.
-  eapply type_L in H.
-  rewrite id_subst__id in H; [|apply id_subst_is_IdSubst].
+Theorem strong_normalization_gu Δ s T : Δ |-* s : T -> @sn term step_gu s.
+  intros Hkind.
+  eapply type_L in Hkind.
+  rewrite id_subst__id in Hkind; [|apply id_subst_is_IdSubst].
   eapply L_sn; eauto.
 Qed.
-
-(* Print Assumptions SN_gu. *)
